@@ -32,6 +32,21 @@ public def Assignment.setElem {v} {α : Nat → Type} [Domain α]
   let map := a.inner.insert index value
   { inner := map, membership := by simp[map, a.membership] }
 
+public theorem Assignment.eq_getElem {v} {α : Nat → Type} [Domain α]
+  (a b: Assignment v α) : a = b ↔ ∀ i : Fin v.size, a.getElem i = b.getElem i := by
+  rw[Assignment.mk.injEq]
+  apply Iff.intro
+  { intro h; simp[getElem,h] }
+  {
+    intro h
+    ext i hI
+    simp[getElem] at h
+    let h := h i
+    rw (occs := .pos [1,2])[← Option.some.injEq] at h
+    repeat rw [← Std.ExtDHashMap.get?_eq_some_get] at h
+    simp[h]
+  }
+
 
 public theorem Assignment.setElem_getElem_previous {v} {α : Nat → Type} [Domain α]
   (a: Assignment v α) (s p: (Fin v.size)) (val: (α ∘ v.varWidth) s)
@@ -89,7 +104,6 @@ public theorem Assignment.γ_elem {v} {α : Nat → Type} [Domain α] [AbstractD
   : a.γ c → AbstractDomain.γ (a.getElem i) (c.getElem i) := by
   intro h; exact Iff.mp (Assignment.γ_forall a c) h i
 
-
 public def Assignment.split {v} {α} [Domain α] [AbstractDomain α]
   (a: Assignment v α) (varIndex: Fin v.size) (bitIndex: Fin (v.varWidth varIndex))
   : (Assignment v α) × (Assignment v α) :=
@@ -101,6 +115,24 @@ public def Assignment.split {v} {α} [Domain α] [AbstractDomain α]
     (leftAssignment, rightAssignment)
 
 -- functions to make assignments
+
+public def Assignment.choice {v} {α : Nat → Type} [Domain α] [AbstractDomain α]
+  (a: Assignment v α) : { c: Assignment v Bitvector // a.γ c} :=
+  let map: Std.ExtDHashMap (Fin v.size) (Bitvector ∘ VarWidths.varWidth v) :=
+    a.inner.map λ k v => (AbstractDomain.choice v).val
+
+  let membership := by simp[a.membership]
+
+  let chosen := { inner := map, membership }
+  let h := by
+    simp[chosen, map]
+    rw[Assignment.γ_forall]
+    intro i
+    simp[getElem, AbstractDomain.choice_within]
+  Subtype.mk chosen h
+
+public theorem Assignment.choice_within {v} {α} [Domain α] [AbstractDomain α] (a: Assignment v α)
+  : γ (a) (choice a).val = true := by simp[(Assignment.choice a).property]
 
 public def Assignment.createFromFn (α) [Domain α] (v: VarWidths)
   (fn : (n: Fin v.size) → α (v.varWidth n)) : Assignment v α :=
